cleaned up semtyping and commented. broke something in soundness

semtyping.v
@@ -3,6 +3,17 @@ From WR Require Import syntax join imports.
 Definition ProdSpace (PA : tm -> Prop) (PF : tm -> (tm -> Prop) -> Prop) (b : tm) :=
   forall a PB, PA a -> PF a PB -> PB (tApp b a).
 
+(* Logical Relation: 
+
+  InterpUnivN i A P  holds when 
+   - A is a Set i 
+   - P is a predicate on terms that act like type A
+
+  We define this in two parts: one that generalizes over
+  smaller interpretations and then tie the knot
+  with the real definition below.
+
+ *)
 Inductive InterpExt n (I : nat -> tm -> Prop) : tm -> (tm -> Prop) -> Prop :=
 | InterpExt_Void : InterpExt n I tVoid (const False)
 | InterpExt_Bool : InterpExt n I tBool (fun a => exists v, Pars a v /\ is_bool_val v)
@@ -11,56 +22,111 @@ Inductive InterpExt n (I : nat -> tm -> Prop) : tm -> (tm -> Prop) -> Prop :=
   (forall a, PA a -> exists PB, PF a PB) ->
   (forall a PB, PF a PB -> InterpExt n I (subst_tm (a..) B) PB) ->
   InterpExt n I (tPi A B) (ProdSpace PA PF)
-| InterpExt_Univ m :
+| InterpExt_Univ m PA :
   m < n ->
-  InterpExt n I (tUniv m) (I m)
-| InterpExt_Eq a b A :
-  InterpExt n I (tEq a b A) (fun p => Pars p tRefl /\ Coherent a b)
+  PA = I m ->
+  InterpExt n I (tUniv m) PA
+| InterpExt_Eq a b A PA :
+  PA = (fun p => Pars p tRefl /\ Coherent a b) ->
+  InterpExt n I (tEq a b A) PA
 | InterpExt_Step A A0 PA :
   Par A A0 ->
   InterpExt n I A0 PA ->
   InterpExt n I A PA.
 
-Lemma InterpExt_Fun_nopf n I A B PA  :
-  InterpExt n I A PA ->
-  (forall a, PA a -> exists PB, InterpExt n I (subst_tm (a..) B) PB) ->
-  InterpExt n I (tPi A B) (ProdSpace PA (fun a => InterpExt n I (subst_tm (a..) B))).
-Proof.
-  move => h0 h1. apply InterpExt_Fun =>//.
-Qed.
-
-Lemma InterpExt_Eq' n I PA a b A :
-  PA = (fun p => Pars p tRefl /\ Coherent a b) ->
-  InterpExt n I (tEq a b A) PA.
-Proof. hauto lq:on use:InterpExt_Eq. Qed.
-
-Lemma InterpExt_Univ' n I m PF :
-  PF = I m ->
-  m < n ->
-  InterpExt n I (tUniv m) PF.
-Proof. hauto lq:on ctrs:InterpExt. Qed.
 
 Equations InterpUnivN (n : nat) : tm -> (tm -> Prop) -> Prop by wf n lt :=
-  InterpUnivN n := InterpExt n (fun m A =>
-                                  match Compare_dec.lt_dec m n with
-                                  | left h => exists PA, InterpUnivN m A PA
-                                  | right _ => False
-                                  end).
+  InterpUnivN n := 
+    InterpExt n (fun m A =>
+                   match Compare_dec.lt_dec m n with
+                   | left h => exists PA, InterpUnivN m A PA
+                   | right _ => False
+                   end).
 
-Lemma InterpExt_Fun_inv n I A B P  (h : InterpExt n I (tPi A B) P) :
-  exists (PA : tm -> Prop) (PF : tm -> (tm -> Prop) -> Prop),
-    InterpExt n I A PA /\
-    (forall a, PA a -> exists PB, PF a PB) /\
-    (forall a PB, PF a PB -> InterpExt n I (subst_tm (a..) B) PB) /\
-    P = ProdSpace PA PF.
+(* ---------------------------------------------------- *)
+
+(* The definition of InterpUnivN is more complicated than 
+   it needs to be. We show that that we can 
+   simplify the unfolding above to just mention InterpUnivN
+   without doing the case analysis.
+*)
+
+Lemma InterpExt_lt_redundant n I A PA
+  (h : InterpExt n I A PA) :
+      InterpExt n (fun m A =>
+                     match Compare_dec.lt_dec m n with
+                     | left h => I m A
+                     | right _ => False
+                     end) A PA.
 Proof.
-  move E : (tPi A B) h => T h.
-  move : A B E.
-  elim : T P / h => //.
+  elim : A PA / h.
   - hauto l:on.
-  - move => *; subst.
-    hauto lq:on inv:Par ctrs:InterpExt use:par_subst.
+  - hauto l:on.
+  - hauto l:on ctrs:InterpExt.
+  - move => m h h1 h2.
+    apply InterpExt_Univ; auto.
+    case : Compare_dec.lt_dec => //.
+  - hauto l:on ctrs:InterpExt.
+  - hauto lq:on ctrs:InterpExt.
 Qed.
+
+Lemma InterpExt_lt_redundant2 n I A PA
+  (h : InterpExt n (fun m A =>
+                      match Compare_dec.lt_dec m n with
+                     | left h => I m A
+                     | right _ => False
+                     end) A PA) :
+  InterpExt n I A PA.
+Proof.
+  elim : A PA / h.
+  - hauto l:on.
+  - hauto l:on.
+  - hauto l:on ctrs:InterpExt.
+  - move => m PA ? ? .
+    eapply InterpExt_Univ => //. subst.
+    case : Compare_dec.lt_dec => //.
+  - hauto l:on ctrs:InterpExt.
+  - hauto lq:on ctrs:InterpExt.
+Qed.
+
+Lemma InterpUnivN_nolt n :
+  InterpUnivN n = InterpExt n (fun m A => exists PA, InterpUnivN m A PA).
+Proof.
+  simp InterpUnivN.
+  fext => A P.
+  apply propositional_extensionality.
+  hauto l:on use:InterpExt_lt_redundant, InterpExt_lt_redundant2.
+Qed.
+
+#[export]Hint Rewrite InterpUnivN_nolt : InterpUniv.
+
+(* For all of the proofs about InterpUnivN below, we need to 
+   do them in two steps. Once for InterpExt, and then tie the 
+   knot for the full definition. *)
+
+(* --------------- relation is cumulative ----------------- *)
+
+Lemma InterpExt_cumulative n m I A PA :
+  n < m ->
+  InterpExt n I A PA ->
+  InterpExt m I A PA.
+Proof.
+  move => h h0.
+  elim : A PA /h0;
+    hauto l:on ctrs:InterpExt use:PeanoNat.Nat.lt_trans.
+Qed.
+
+Lemma InterpUnivN_cumulative n A PA :
+  InterpUnivN n A PA -> forall m, n < m ->
+  InterpUnivN m A PA.
+Proof.
+  hauto l:on rew:db:InterpUniv use:InterpExt_cumulative.
+Qed.
+
+(* ------------------------------------------------------- *)
+
+(* The logical relation is closed under parallel reduction, 
+   forwards and backwards. *)
 
 Lemma InterpExt_preservation n I A B P (h : InterpExt n I A P) :
   Par A B ->
@@ -78,9 +144,9 @@ Proof.
     apply : ihPB; eauto.
     sfirstorder use:par_cong, Par_refl.
   - hauto lq:on inv:Par ctrs:InterpExt.
-  - move => a b A B.
+  - move => a b A B PA EQ.
     elim /Par_inv=>// h ? ? ? a0 b0 A0 ? ? ? [] *. subst.
-    apply InterpExt_Eq'.
+    eapply InterpExt_Eq.
     fext => p.
     f_equal.
     apply propositional_extensionality.
@@ -100,6 +166,11 @@ Lemma InterpExt_back_preservation_star i I A B P (h : InterpExt i I B P) :
   InterpExt i I A P.
 Proof. induction 1; hauto l:on ctrs:InterpExt. Qed.
 
+Lemma InterpUnivN_back_preservation_star n A B P (h : InterpUnivN n B P) :
+  Pars A B ->
+  InterpUnivN n A P.
+Proof. hauto l:on rew:db:InterpUnivN use:InterpExt_back_preservation_star. Qed.
+
 Lemma InterpExt_preservation_star n I A B P (h : InterpExt n I A P) :
   Pars A B ->
   InterpExt n I B P.
@@ -110,16 +181,26 @@ Lemma InterpUnivN_preservation_star n A B P (h : InterpUnivN n A P) :
   InterpUnivN n B P.
 Proof. hauto l:on rew:db:InterpUnivN use:InterpExt_preservation_star. Qed.
 
-Lemma InterpUnivN_back_preservation_star n A B P (h : InterpUnivN n B P) :
-  Pars A B ->
-  InterpUnivN n A P.
-Proof. hauto l:on rew:db:InterpUnivN use:InterpExt_back_preservation_star. Qed.
+(* ---------------------------------------------------------- *)
 
 Lemma InterpUnivN_Coherent n A B P (h : InterpUnivN n B P) :
   Coherent A B ->
   InterpUnivN n A P.
 Proof.
   hauto l:on unfold:Coherent use:InterpUnivN_back_preservation_star, InterpUnivN_preservation_star.
+Qed.
+
+(* ---------------------------------------------------------- *)
+(* inversion lemmas for InterpExt. To invert the InterpExt 
+   judgment, we have to be careful about the step case. *)
+
+Lemma InterpExt_Void_inv n I P :
+  InterpExt n I tVoid P ->
+  P = (const False).
+Proof.
+  move E : tVoid => A h.
+  move : E.
+  elim : A P / h; hauto lq:on inv:Par.
 Qed.
 
 Lemma InterpExt_Bool_inv n I P :
@@ -131,13 +212,19 @@ Proof.
   elim : A P / h; hauto lq:on inv:Par.
 Qed.
 
-Lemma InterpExt_Void_inv n I P :
-  InterpExt n I tVoid P ->
-  P = (const False).
+Lemma InterpExt_Fun_inv n I A B P  (h : InterpExt n I (tPi A B) P) :
+  exists (PA : tm -> Prop) (PF : tm -> (tm -> Prop) -> Prop),
+    InterpExt n I A PA /\
+    (forall a, PA a -> exists PB, PF a PB) /\
+    (forall a PB, PF a PB -> InterpExt n I (subst_tm (a..) B) PB) /\
+    P = ProdSpace PA PF.
 Proof.
-  move E : tVoid => A h.
-  move : E.
-  elim : A P / h; hauto lq:on inv:Par.
+  move E : (tPi A B) h => T h.
+  move : A B E.
+  elim : T P / h => //.
+  - hauto l:on.
+  - move => *; subst.
+    hauto lq:on inv:Par ctrs:InterpExt use:par_subst.
 Qed.
 
 Lemma InterpExt_Univ_inv n I P m :
@@ -148,11 +235,6 @@ Proof.
   move : E.
   elim : A P / h; hauto lq:on rew:off inv:Par.
 Qed.
-
-Lemma InterpUnivN_Bool_inv n P :
-  InterpUnivN n tBool P ->
-  P = fun a => exists v, Pars a v /\ is_bool_val v.
-Proof. hauto l:on rew:db:InterpUnivN use:InterpExt_Bool_inv. Qed.
 
 Lemma InterpExt_Eq_inv n I a b A P :
   InterpExt n I (tEq a b A) P ->
@@ -170,6 +252,8 @@ Proof.
   apply propositional_extensionality.
   hauto lq:on use:Par_Coherent, Coherent_symmetric, Coherent_transitive.
 Qed.
+
+(* ------------- relation is deterministic ---------------- *)
 
 Lemma InterpExt_deterministic n I A PA PB :
   InterpExt n I A PA ->
@@ -193,6 +277,61 @@ Proof.
   - hauto l:on use:InterpExt_preservation.
 Qed.
 
+
+Lemma InterpUnivN_deterministic n A PA PB :
+  InterpUnivN n A PA ->
+  InterpUnivN n A PB ->
+  PA = PB.
+Proof.
+  simp InterpUnivN.
+  eauto using InterpExt_deterministic.
+Qed.
+
+(* slight generalization to work with any levels. *)
+
+Lemma InterpExt_deterministic' n m I A PA PB :
+  InterpExt n I A PA ->
+  InterpExt m I A PB ->
+  PA = PB.
+Proof.
+  move => h0 h1.
+  case : (Coq.Arith.Compare_dec.lt_eq_lt_dec m n); first case.
+  - hauto l:on use:InterpExt_cumulative, InterpExt_deterministic.
+  - move => *; subst.
+    sfirstorder use:InterpExt_deterministic.
+  - move => ?.
+    symmetry.
+    hauto l:on use:InterpExt_cumulative, InterpExt_deterministic.
+Qed.
+
+
+Lemma InterpUnivN_deterministic' n m  A PA PB :
+  InterpUnivN n A PA ->
+  InterpUnivN m A PB ->
+  PA = PB.
+Proof. hauto lq:on rew:off use:InterpExt_deterministic' rew:db:InterpUniv. Qed.
+
+
+(* ---------------------------------------------------------- *)
+
+Lemma InterpExt_Fun_nopf n I A B PA  :
+  InterpExt n I A PA ->
+  (forall a, PA a -> exists PB, InterpExt n I (subst_tm (a..) B) PB) ->
+  InterpExt n I (tPi A B) (ProdSpace PA (fun a => InterpExt n I (subst_tm (a..) B))).
+Proof.
+  move => h0 h1. apply InterpExt_Fun =>//.
+Qed.
+
+(* should this be called InterpUnivN_Fun_nopf ? *)
+Lemma InterpUnivN_Fun n A B PA :
+  InterpUnivN n A PA ->
+  (forall a, PA a -> exists PB, InterpUnivN n (subst_tm (a..) B) PB) ->
+  InterpUnivN n (tPi A B) (ProdSpace PA (fun a => InterpUnivN n (subst_tm (a..) B))).
+Proof.
+  hauto l:on use:InterpExt_Fun_nopf rew:db:InterpUniv.
+Qed.
+
+
 Lemma InterpExt_Fun_inv_nopf n I A B P  (h : InterpExt n I (tPi A B) P) :
   exists (PA : tm -> Prop),
     InterpExt n I A PA /\
@@ -210,82 +349,6 @@ Proof.
     + sfirstorder.
 Qed.
 
-Lemma InterpUnivN_deterministic n A PA PB :
-  InterpUnivN n A PA ->
-  InterpUnivN n A PB ->
-  PA = PB.
-Proof.
-  simp InterpUnivN.
-  eauto using InterpExt_deterministic.
-Qed.
-
-Lemma InterpExt_cumulative n m I A PA :
-  n < m ->
-  InterpExt n I A PA ->
-  InterpExt m I A PA.
-Proof.
-  move => h h0.
-  elim : A PA /h0;
-    hauto l:on ctrs:InterpExt use:PeanoNat.Nat.lt_trans.
-Qed.
-
-Lemma InterpExt_lt_redundant n I A PA
-  (h : InterpExt n I A PA) :
-      InterpExt n (fun m A =>
-                     match Compare_dec.lt_dec m n with
-                     | left h => I m A
-                     | right _ => False
-                     end) A PA.
-Proof.
-  elim : A PA / h.
-  - hauto l:on.
-  - hauto l:on.
-  - hauto l:on ctrs:InterpExt.
-  - move => m h.
-    apply InterpExt_Univ' => //.
-    case : Compare_dec.lt_dec => //.
-  - hauto l:on.
-  - hauto lq:on ctrs:InterpExt.
-Qed.
-
-Lemma InterpExt_lt_redundant2 n I A PA
-  (h : InterpExt n (fun m A =>
-                      match Compare_dec.lt_dec m n with
-                     | left h => I m A
-                     | right _ => False
-                     end) A PA) :
-  InterpExt n I A PA.
-Proof.
-  elim : A PA / h.
-  - hauto l:on.
-  - hauto l:on.
-  - hauto l:on ctrs:InterpExt.
-  - move => m ?.
-    apply InterpExt_Univ' => //.
-    case : Compare_dec.lt_dec => //.
-  - hauto l:on.
-  - hauto lq:on ctrs:InterpExt.
-Qed.
-
-Lemma InterpUnivN_nolt n :
-  InterpUnivN n = InterpExt n (fun m A => exists PA, InterpUnivN m A PA).
-Proof.
-  simp InterpUnivN.
-  fext => A P.
-  apply propositional_extensionality.
-  hauto l:on use:InterpExt_lt_redundant, InterpExt_lt_redundant2.
-Qed.
-
-#[export]Hint Rewrite InterpUnivN_nolt : InterpUniv.
-
-Lemma InterpUnivN_Fun n A B PA :
-  InterpUnivN n A PA ->
-  (forall a, PA a -> exists PB, InterpUnivN n (subst_tm (a..) B) PB) ->
-  InterpUnivN n (tPi A B) (ProdSpace PA (fun a => InterpUnivN n (subst_tm (a..) B))).
-Proof.
-  hauto l:on use:InterpExt_Fun_nopf rew:db:InterpUniv.
-Qed.
-
 Lemma InterpUnivN_Fun_inv_nopf n A B P  (h : InterpUnivN n (tPi A B) P) :
   exists (PA : tm -> Prop),
     InterpUnivN n A PA /\
@@ -295,33 +358,38 @@ Proof.
   qauto use:InterpExt_Fun_inv_nopf l:on rew:db:InterpUniv.
 Qed.
 
-Lemma InterpExt_deterministic' n m I A PA PB :
-  InterpExt n I A PA ->
-  InterpExt m I A PB ->
-  PA = PB.
+(* ------- construction and inversion lemmas for InterpUnivN -------------- *)
+
+Lemma InterpUnivN_Bool_inv n P :
+  InterpUnivN n tBool P ->
+  P = fun a => exists v, Pars a v /\ is_bool_val v.
+Proof. hauto l:on rew:db:InterpUnivN use:InterpExt_Bool_inv. Qed.
+
+Lemma InterpUnivN_Univ i j :
+  j < i ->
+  InterpUnivN i (tUniv j) (fun A : tm => exists (PA : tm -> Prop), InterpUnivN j A PA).
 Proof.
-  move => h0 h1.
-  case : (Coq.Arith.Compare_dec.lt_eq_lt_dec m n); first case.
-  - hauto l:on use:InterpExt_cumulative, InterpExt_deterministic.
-  - move => *; subst.
-    sfirstorder use:InterpExt_deterministic.
-  - move => ?.
-    symmetry.
-    hauto l:on use:InterpExt_cumulative, InterpExt_deterministic.
+  move => hji.
+  simp InterpUniv.
+  apply InterpExt_Univ => [|//]; auto.
+  by simp InterpUniv.
 Qed.
 
-Lemma InterpUnivN_cumulative n A PA :
-  InterpUnivN n A PA -> forall m, n < m ->
-  InterpUnivN m A PA.
+Lemma InterpUnivN_Univ_inv' i j P :
+  InterpUnivN i (tUniv j) P ->
+  P = (fun A : tm => exists (PA : tm -> Prop), InterpUnivN j A PA) /\ j < i.
 Proof.
-  hauto l:on rew:db:InterpUniv use:InterpExt_cumulative.
+  hauto q:on rew:db:InterpUniv use:InterpExt_Univ_inv.
 Qed.
 
-Lemma InterpUnivN_deterministic' n m  A PA PB :
-  InterpUnivN n A PA ->
-  InterpUnivN m A PB ->
-  PA = PB.
-Proof. hauto lq:on rew:off use:InterpExt_deterministic' rew:db:InterpUniv. Qed.
+Lemma InterpUnivN_Eq n a b A :
+  InterpUnivN n (tEq a b A) (fun p => Pars p tRefl /\ Coherent a b).
+Proof. 
+  simp InterpUniv.
+  apply InterpExt_Eq => [//]; auto.
+Qed.
+
+(* ------------ More closure under Par -------------- *)
 
 Lemma InterpExt_back_clos n I A PA
   (hI : forall m, m < n -> forall A B, Par A B -> I m B -> I m A):
@@ -338,14 +406,13 @@ Proof.
     have ? : Par (tApp b0 a)(tApp b1 a) by hauto lq:on ctrs:Par use:Par_refl.
     hauto lq:on ctrs:Par.
   - hauto lq:on.
-  - hauto lq:on ctrs:rtc.
+  - move => a b T PA ->. hauto lq:on ctrs:rtc.
   - sfirstorder.
 Qed.
 
 Lemma InterpUnivN_back_clos n A PA :
     InterpUnivN n A PA ->
-    forall a b, Par a b ->
-           PA b -> PA a.
+    forall a b, Par a b -> PA b -> PA a.
 Proof.
   simp InterpUniv.
   apply InterpExt_back_clos.
@@ -361,19 +428,6 @@ Proof.
   induction 1; sfirstorder use:InterpUnivN_back_clos.
 Qed.
 
-Lemma InterpUnivN_Univ_inv i j :
-  j < i ->
-  InterpUnivN i (tUniv j) (fun A : tm => exists (PA : tm -> Prop), InterpUnivN j A PA).
-Proof.
-  move => hji.
-  simp InterpUniv.
-  apply InterpExt_Univ' => [|//].
-  by simp InterpUniv.
-Qed.
 
-Lemma InterpUnivN_Univ_inv' i j P :
-  InterpUnivN i (tUniv j) P ->
-  P = (fun A : tm => exists (PA : tm -> Prop), InterpUnivN j A PA) /\ j < i.
-Proof.
-  hauto q:on rew:db:InterpUniv use:InterpExt_Univ_inv.
-Qed.
+
+
